refactored syntax

formalization/code/Containers_Code.thy
@@ -1,19 +1,12 @@
 theory Containers_Code
-imports Monitor_Code Containers.Containers Deriving.Derive
+imports Whymon.Monitor Containers.Containers Deriving.Derive
 begin
-
-
 
 derive (eq) ceq event_data
 derive ccompare event_data
 derive (eq) ceq string8
 derive (linorder) compare string8
 derive (compare) ccompare string8
-instantiation event_data :: card_UNIV begin
-definition "finite_UNIV = Phantom(event_data) False"
-definition "card_UNIV = Phantom(event_data) 0"
-instance by intro_classes (simp_all add: finite_UNIV_event_data_def card_UNIV_event_data_def infinite_UNIV_event_data)
-end
 
 subsection \<open>Comparator\<close>
 
