formalization/thys/Proof_Object.thy
@@ -1,0 +1,119 @@
+theory Proof_Object
+imports Proof_System Partition
+begin
+
+subsection \<open>Proof Objects\<close>
+
+datatype (dead 'd) sproof = STT nat 
+  | SPred nat Formula.name "'d Formula.trm list"
+  | SEq_Const nat Formula.name 'd
+  | SNeg "'d vproof" 
+  | SOrL "'d sproof" 
+  | SOrR "'d sproof" 
+  | SAnd "'d sproof" "'d sproof"
+  | SImpL "'d vproof" 
+  | SImpR "'d sproof"
+  | SIffSS "'d sproof" "'d sproof" 
+  | SIffVV "'d vproof" "'d vproof" 
+  | SExists Formula.name 'd "'d sproof"
+  | SForall Formula.name "('d, 'd sproof) part" 
+  | SPrev "'d sproof"
+  | SNext "'d sproof"
+  | SOnce nat "'d sproof"
+  | SEventually nat "'d sproof" 
+  | SHistorically nat nat "'d sproof list" 
+  | SHistoricallyOut nat
+  | SAlways nat nat "'d sproof list"
+  | SSince "'d sproof" "'d sproof list" 
+  | SUntil "'d sproof list" "'d sproof" 
+  and 'd vproof = VFF nat 
+  | VPred nat Formula.name "'d Formula.trm list"
+  | VEq_Const nat Formula.name 'd
+  | VNeg "'d sproof" 
+  | VOr "'d vproof" "'d vproof"
+  | VAndL "'d vproof" 
+  | VAndR "'d vproof" 
+  | VImp "'d sproof" "'d vproof" 
+  | VIffSV "'d sproof" "'d vproof" 
+  | VIffVS "'d vproof" "'d sproof" 
+  | VExists Formula.name "('d, 'd vproof) part" 
+  | VForall Formula.name 'd "'d vproof"
+  | VPrev "'d vproof"
+  | VPrevZ
+  | VPrevOutL nat 
+  | VPrevOutR nat
+  | VNext "'d vproof" 
+  | VNextOutL nat 
+  | VNextOutR nat 
+  | VOnceOut nat 
+  | VOnce nat nat "'d vproof list" 
+  | VEventually nat nat "'d vproof list"
+  | VHistorically nat "'d vproof" 
+  | VAlways nat "'d vproof"
+  | VSinceOut nat
+  | VSince nat "'d vproof" "'d vproof list" 
+  | VSinceInf nat nat "'d vproof list" 
+  | VUntil nat "'d vproof list" "'d vproof"
+  | VUntilInf nat nat "'d vproof list"
+
+type_synonym 'd "proof" = "'d sproof + 'd vproof"
+
+type_synonym 'd expl = "('d, 'd proof, Formula.name) pdt"
+
+fun s_at :: "'d sproof \<Rightarrow> nat" and 
+  v_at :: "'d vproof \<Rightarrow> nat" where
+  "s_at (STT i) = i"
+| "s_at (SPred i _ _) = i"
+| "s_at (SEq_Const i _ _) = i"
+| "s_at (SNeg vp) = v_at vp"
+| "s_at (SOrL sp1) = s_at sp1"
+| "s_at (SOrR sp2) = s_at sp2"
+| "s_at (SAnd sp1 _) = s_at sp1"
+| "s_at (SImpL vp1) = v_at vp1"
+| "s_at (SImpR sp2) = s_at sp2"
+| "s_at (SIffSS sp1 _) = s_at sp1"
+| "s_at (SIffVV vp1 _) = v_at vp1"
+| "s_at (SExists _ _ sp) = s_at sp"
+| "s_at (SForall _ part) = s_at (part_hd part)"
+| "s_at (SPrev sp) = s_at sp + 1"
+| "s_at (SNext sp) = s_at sp - 1"
+| "s_at (SOnce i _) = i"
+| "s_at (SEventually i _) = i"
+| "s_at (SHistorically i _ _) = i"
+| "s_at (SHistoricallyOut i) = i"
+| "s_at (SAlways i _ _) = i"
+| "s_at (SSince sp2 sp1s) = (case sp1s of [] \<Rightarrow> s_at sp2 | _ \<Rightarrow> s_at (last sp1s))"
+| "s_at (SUntil sp1s sp2) = (case sp1s of [] \<Rightarrow> s_at sp2 | sp1 # _ \<Rightarrow> s_at sp1)"
+| "v_at (VFF i) = i"
+| "v_at (VPred i _ _) = i"
+| "v_at (VEq_Const i _ _) = i"
+| "v_at (VNeg sp) = s_at sp"
+| "v_at (VOr vp1 _) = v_at vp1"
+| "v_at (VAndL vp1) = v_at vp1"
+| "v_at (VAndR vp2) = v_at vp2"
+| "v_at (VImp sp1 _) = s_at sp1"
+| "v_at (VIffSV sp1 _) = s_at sp1"
+| "v_at (VIffVS vp1 _) = v_at vp1"
+| "v_at (VExists _ part) = v_at (part_hd part)"
+| "v_at (VForall _ _ vp1) = v_at vp1"
+| "v_at (VPrev vp) = v_at vp + 1"
+| "v_at (VPrevZ) = 0"
+| "v_at (VPrevOutL i) = i"
+| "v_at (VPrevOutR i) = i"
+| "v_at (VNext vp) = v_at vp - 1"
+| "v_at (VNextOutL i) = i"
+| "v_at (VNextOutR i) = i"
+| "v_at (VOnceOut i) = i"
+| "v_at (VOnce i _ _) = i"
+| "v_at (VEventually i _ _) = i"
+| "v_at (VHistorically i _) = i"
+| "v_at (VAlways i _) = i"
+| "v_at (VSinceOut i) = i"
+| "v_at (VSince i _ _) = i"
+| "v_at (VSinceInf i _ _) = i"
+| "v_at (VUntil i _ _) = i"
+| "v_at (VUntilInf i _ _) = i"
+
+definition p_at :: "'d proof \<Rightarrow> nat" where "p_at p = case_sum s_at v_at p" 
+
+end
